code/blake2/Hacl.Impl.Blake2.FGeneric.fst
@@ -1,0 +1,79 @@
+module Hacl.Impl.Blake2.FGeneric
+
+open FStar.Mul
+open FStar.HyperStack
+open FStar.HyperStack.ST
+
+open Lib.IntTypes
+open Lib.Buffer
+open Lib.ByteBuffer
+open Lib.LoopCombinators
+
+module ST = FStar.HyperStack.ST
+module Seq = Lib.Sequence
+module Loops = Lib.LoopCombinators
+module Spec = Spec.Blake2
+
+open Hacl.Impl.Blake2.Constants
+open Hacl.Impl.Blake2.Core
+open Hacl.Impl.Blake2.Generic
+module Blake2s32 = Hacl.Blake2s_32
+module Blake2s128 = Hacl.Blake2s_128
+module Blake2b32 = Hacl.Blake2b_32
+module Blake2b256 = Hacl.Blake2b_256
+
+#set-options "--z3rlimit 50 --max_ifuel 0 --max_fuel 0"
+
+/// FGeneric: factorized generic.
+/// The generic implementation of Blake2, but relying on intermediate definitions.
+/// Allows to factorize code between the one-shot hash and the generic hash.
+
+noextract
+let is_valid_m_spec (al : Spec.alg) (ms : m_spec) =
+  match al, ms with
+  | Spec.Blake2S, M32
+  | Spec.Blake2S, M128
+  | Spec.Blake2B, M32
+  | Spec.Blake2B, M256 -> true
+  | _ -> false
+
+inline_for_extraction noextract
+let valid_m_spec (al : Spec.alg) = ms:m_spec{is_valid_m_spec al ms}
+
+inline_for_extraction noextract
+let blake2_init (#al : Spec.alg) (#ms : valid_m_spec al) : blake2_init_st al ms =
+  match al, ms with
+  | Spec.Blake2S, M32 -> Blake2s32.blake2s_init
+  | Spec.Blake2S, M128 -> Blake2s128.blake2s_init
+  | Spec.Blake2B, M32 -> Blake2b32.blake2b_init
+  | Spec.Blake2B, M256 -> Blake2b256.blake2b_init
+
+inline_for_extraction noextract
+let blake2_update_multi (#al : Spec.alg) (#ms : valid_m_spec al) :
+  blake2_update_multi_st al ms =
+  match al, ms with
+  | Spec.Blake2S, M32 -> Blake2s32.blake2s_update_multi
+  | Spec.Blake2S, M128 -> Blake2s128.blake2s_update_multi
+  | Spec.Blake2B, M32 -> Blake2b32.blake2b_update_multi
+  | Spec.Blake2B, M256 -> Blake2b256.blake2b_update_multi
+
+inline_for_extraction noextract
+let blake2_update_last (#al : Spec.alg) (#ms : valid_m_spec al) :
+  blake2_update_last_st al ms =
+  match al, ms with
+  | Spec.Blake2S, M32 -> Blake2s32.blake2s_update_last
+  | Spec.Blake2S, M128 -> Blake2s128.blake2s_update_last
+  | Spec.Blake2B, M32 -> Blake2b32.blake2b_update_last
+  | Spec.Blake2B, M256 -> Blake2b256.blake2b_update_last
+
+inline_for_extraction noextract
+let blake2_finish (#al : Spec.alg) (#ms : valid_m_spec al) :
+  blake2_finish_st al ms =
+  match al, ms with
+  | Spec.Blake2S, M32 -> Blake2s32.blake2s_finish
+  | Spec.Blake2S, M128 -> Blake2s128.blake2s_finish
+  | Spec.Blake2B, M32 -> Blake2b32.blake2b_finish
+  | Spec.Blake2B, M256 -> Blake2b256.blake2b_finish
+
+
+
